https://leetcode.cn/problems/convert-integer-to-the-sum-of-two-no-zero-integers/description/ 

- Solution 1:
```
public class Solution {
    public int[] GetNoZeroIntegers(int n) {
        var a = 1;
        var b = n - 1;
        if (IsNoZero(b))
            return new int[] { a, b};

        while (true)
        {
            a += 1;
            b -= 1;
            if (IsNoZero(a) && IsNoZero(b))
                break;
        }
        return new int[] { a, b };
    }

    private bool IsNoZero(int x)
    {
        var str = x.ToString();
        return str.IndexOf('0') < 0;
    }
}
```
**Python**
```
class Solution:
    def getNoZeroIntegers(self, n: int) -> List[int]:
        def isNoZero(x: int):
            str_x = str(x)
            return '0' not in str_x
        a, b = 1, n - 1
        if isNoZero(b):
            return [a, b]
        while True:
            a += 1
            b -= 1
            if isNoZero(a) and isNoZero(b):
                break
        return [a, b]

        
```

---

- Solution 2: (Recommendation)
```
public class Solution {
    public int[] GetNoZeroIntegers(int n) {
        for (var a = 1; a < n; a++)
        {
            var b = n - a;
            if ((a.ToString() + b.ToString()).IndexOf('0') < 0)
                return new int[] { a, b };
        }
        return new int[] {};
    }
}
```
**Python**
```
class Solution:
    def getNoZeroIntegers(self, n: int) -> List[int]:
        for a in range(1, n):
            b = n - a
            if '0' not in str(a) + str(b):
                return [a, b]
        return []

        
```
